src/Mman.fst
@@ -4,39 +4,41 @@ open Steel.Effect.Atomic
 open Steel.Effect
 module A = Steel.Array
 
-module U64 = FStar.UInt64
-module U32 = FStar.UInt32
-module I32 = FStar.Int32
+//module U64 = FStar.UInt64
+//module U32 = FStar.UInt32
+//module I32 = FStar.Int32
 module U8 = FStar.UInt8
+module US = FStar.SizeT
+//module UP = FStar.PtrdiffT
 
 let array = Steel.ST.Array.array
 
 
 noextract
 assume val mmap
-  (addr: U64.t)
-  (len: U64.t)
-  (prot: I32.t)
-  (flags: I32.t)
-  (fildes: I32.t)
-  (off: U32.t)
+  //(addr: U64.t)//TODO: implicit cast
+  (size: US.t)
+  //(prot: I32.t)
+  //(flags: I32.t)
+  //(fd: I32.t)
+  //(off: U32.t)
   : Steel (array U8.t)
     emp
     (fun a -> A.varray a)
-    (fun _ -> True)
-    (fun _ a h1 ->
-      A.length a == U64.v len /\
+    (requires fun _ -> True)
+    (ensures fun _ a h1 ->
+      A.length a == US.v size /\
       A.is_full_array a /\
-      A.asel a h1 == Seq.create (U64.v len) U8.zero
+      A.asel a h1 == Seq.create (US.v size) U8.zero
     )
 
 noextract
-assume val munmap (a: array U8.t) (size_t: U64.t)
-  : Steel unit
-    (A.varray a)
-    (fun _ -> emp)
-    (fun _ ->
-      A.length a == U64.v size_t /\
-      A.is_full_array a
+assume val munmap (ptr: array U8.t) (size: US.t)
+  : Steel bool
+    (A.varray ptr)
+    (fun b -> if b then emp else A.varray ptr)
+    (requires fun _ ->
+      //A.length a == U64.v size_t /\
+      A.is_full_array ptr
     )
-    (fun _ _ _ -> True)
+    (ensures fun _ _ _ -> True)
